more

Test.c
@@ -41,7 +41,8 @@ bool Test_parse_len(uint8_t *buf, uint32_t len, uint32_t *out_len)
         else
         {
           uint8_t *lbytes = buf + (uint32_t )1;
-          ite = Test_read_length(lbytes, ilen1);
+          uint32_t tmp = Test_read_length(lbytes, ilen1);
+          ite = tmp;
         }
         ite1 = ite;
       }
