test.fst
@@ -13,16 +13,17 @@ module U32 = FStar.UInt32
 
 
 private (* HACL* -> FStar.Endianness *)
-let rec big_endian (b:FStar.Seq.seq U8.t) : Tot nat (decreases (FStar.Seq.length b)) =
+let rec big_endian (b:Seq.seq U8.t) : Tot nat (decreases (FStar.Seq.length b)) =
   let open FStar.Seq in
   if length b = 0 then 0
   else
     U8.v (last b) + pow2 8 * big_endian (slice b 0 (length b - 1))
 
 private
-val big_endian_zero: len:nat{len <= 4} -> Lemma
+val big_endian_zero: len:nat -> Lemma
   (ensures (big_endian (Seq.create len 0uy) == 0))
   (decreases (len))
+  [SMTPat (big_endian (Seq.create len 0uy))]
 let rec big_endian_zero len =
   let open FStar.Seq in
   if len = 0 then ()
@@ -43,11 +44,67 @@ let big_endian_single n =
 
 
 
+private
+let read_length_success (b:Seq.seq U8.t{Seq.length b > 0}) : Tot bool =
+  let open FStar.Seq in
+  let b0 = U8.v (index b 0) in
+  if b0 > 0x80 && b0 < 0x85 && length b > b0 - 0x80 then
+    big_endian (slice b 1 (b0 - 0x80 + 1)) > 0
+  else
+    b0 < 0x80
+
+private // Short form is easy to parse and always succeeds.
+let read_length_success_lemma (b:Seq.seq U8.t{Seq.length b > 0}) : Lemma
+  (requires (U8.v (Seq.index b 0) < 0x80))
+  (ensures (read_length_success b))
+  = ()
+
+private // Fail when given a zero length in long form.
+let read_length_success_lemma2 (b:Seq.seq U8.t{Seq.length b > 0}) : Lemma
+  (requires (U8.v (Seq.index b 0) = 0x80))
+  (ensures (not (read_length_success b)))
+  = ()
+
+private // We can't parse long form with more than 4 bytes.
+let read_length_success_lemma3 (b:Seq.seq U8.t{Seq.length b > 0}) : Lemma
+  (requires (U8.v (Seq.index b 0) > 0x84))
+  (ensures (not (read_length_success b)))
+  = ()
+
+private // The long form must have enough length bytes.
+let read_length_success_lemma4 (b:Seq.seq U8.t{Seq.length b > 0}) : Lemma
+  (requires (U8.v (Seq.index b 0) > 0x80 /\ U8.v (Seq.index b 0) < 0x85) /\ Seq.length b <= (U8.v (Seq.index b 0)) - 0x80)
+  (ensures (not (read_length_success b)))
+  = ()
+
+private // The long form must not be all zero bytes.
+val read_length_success_lemma5: (b:Seq.seq U8.t{Seq.length b > 0}) -> Lemma
+  (requires (U8.v (Seq.index b 0) > 0x80 /\ U8.v (Seq.index b 0) < 0x85 /\
+             Seq.length b > U8.v (Seq.index b 0) - 0x80 /\
+             (forall i. i > 0 /\ i < Seq.length b ==> Seq.index b i = 0uy)))
+  (ensures (not (read_length_success b)))
+let read_length_success_lemma5 b =
+   let len = U8.v (Seq.index b 0) - 0x80 + 1 in
+   assert (Seq.length b >= len /\ len >= 1);
+   Seq.lemma_eq_intro (Seq.slice b 1 len) (Seq.create (len - 1) 0uy);
+   assert (big_endian (Seq.create (len - 1) 0uy) = 0);
+   assert (big_endian (Seq.slice b 1 len) = 0)
+
+(* private
+// Success with long form parsing means we have more than just zero bytes.
+let read_length_success_lemma6 (b:Seq.seq U8.t{Seq.length b > 0}) : Lemma
+  (requires (U8.v (Seq.index b 0) > 0x80 /\ U8.v (Seq.index b 0) < 0x85) /\ Seq.length b > (U8.v (Seq.index b 0)) - 0x80)
+  (ensures (read_length_success b ==> big_endian (Seq.slice b 1 ((Seq.index b 0) - 0x80 + 1)) > 0 /\ b <> (Seq.create (Seq.length b) 0uy)))
+  = () *)
+
+// TODO check long form with starting zero bytes
+
+
 
 val read_length :
   buf:buffer U8.t ->
   len:U32.t{U32.v len <= 4} ->
-  ST (r:U32.t{U32.v r < pow2 (8 * U32.v len)})
+  ST (r:U32.t{U32.v r < pow2 (8 * U32.v len)}) // TODO
   (requires (fun h -> live h buf /\ U32.v len == length buf))
   (ensures (fun h0 r h1 -> h0 == h1 /\ live h1 buf /\ U32.v r == big_endian (as_seq h0 buf)))
   (decreases (length buf))
@@ -61,7 +118,10 @@ let rec read_length buf len =
     let lo = uint8_to_uint32 bi in
     Math.Lemmas.pow2_plus 8 24;
     // TODO assert Buffer.sub
+    //Seq.lemma_eq_intro (as_seq h lbytes) (Seq.slice (as_seq h buf) 1 (U32.v ilen + 1)); // TODO
     let hi = read_length (Buffer.sub buf 0ul len) len in
+    let h = ST.get() in // TODO
+    assert (U32.v hi == big_endian (Seq.slice (as_seq h buf) 0 (U32.v len))); // TODO
     assert (U32.v hi < pow2 (8 * (U32.v len)));
     let hi' = hi <<^ 8ul in
     assert (hi = 0ul ==> hi' = 0ul);
@@ -74,52 +134,6 @@ let rec read_length buf len =
     res
   )
 
-(*
-private // TODO len <= 4
-val test_parse_long_zero : len:U32.t{U32.v len < 2} -> St unit
-
-let rec test_parse_long_zero len = match (U32.v len) with
-  | 0 -> ()
-  | 1 -> (
-      push_frame ();
-      let sdata = Seq.create (U32.v len - 1) 0uy in
-      //let data = create 0uy U32.(len -^ 1ul) in
-      let data = of_seq sdata U32.(len -^ 1ul) in
-      assert (length data = 0);
-      assert (read_length data 0ul = 0ul);
-      //Seq.lemma_index_create (U32.v len - 1) 0uy (U32.v len - 2);
-      let h = ST.get() in
-      Seq.lemma_eq_intro (as_seq h data) (Seq.create (U32.v len - 1) 0uy);
-      assert (read_length data U32.(len -^ 1ul) = 0ul);
-      pop_frame ()
-
-      //push_frame ();
-      //test_parse_long_zero U32.(len -^ 1ul);
-      //let data = create 0uy len in
-      //let h = ST.get() in
-      //Seq.lemma_eq_intro (as_seq h data) (Seq.create (U32.v len) 0uy);
-      //assert (read_length data len = 0ul);
-      //pop_frame ()
-    )
-  *)
-
-  //push_frame ();
-  //let data = create 0uy len in
-  //let h = ST.get() in
-  //Seq.lemma_index_create 1 0x80uy 0;
-  //Seq.lemma_eq_intro (as_seq h data) (Seq.create (U32.v len) 0uy);
-  //assert (get h data 0 = 0uy);
-  //let out_len = create 1ul 1ul in
-  //Seq.lemma_index_create 1 0ul (U32.v len);
-  //let h = ST.get() in
-  //Seq.lemma_eq_intro (as_seq h out_len) (Seq.create 1 1ul);
-  //assert (read_length data len = 0ul);
-  //let h = ST.get() in
-  //assert (not success && get h out_len 0 = 0ul);
-  //assert (get h out_len 0 = 0ul);
-  //Seq.lemma_eq_intro (as_seq h out_len) (Seq.create 1 0ul);
-  //pop_frame ()
-
 
 val parse_len :
   buf:buffer U8.t ->
@@ -128,6 +142,7 @@ val parse_len :
   ST bool
   (requires (fun h -> live h buf /\ live h out_len))
   (ensures (fun h0 r h1 -> live h1 buf /\ live h1 out_len /\
+            //r == read_length_success (as_seq h1 buf) /\ // TODO
             (r \/ (get h1 out_len 0) = 0ul)))
 
 let parse_len buf len out_len =
@@ -161,21 +176,23 @@ let parse_len buf len out_len =
     let lbytes = Buffer.sub buf 1ul ilen in
     let h = ST.get() in // TODO
     Seq.lemma_eq_intro (as_seq h lbytes) (Seq.slice (as_seq h buf) 1 (U32.v ilen + 1));
-    read_length lbytes ilen
+    let tmp = read_length lbytes ilen in // TODO
+    let h = ST.get() in // TODO
+    assert (U32.v tmp == big_endian (Seq.slice (as_seq h buf) 1 (U32.v ilen + 1))); // TODO
+    tmp // TODO
   ) in
 
-  // Write the result. (TODO write without temp var?)
+  // Write the result.
   out_len.(0ul) <- res;
 
   // If we picked a result > 0, success.
   // If the result is 0 because ilen is 0, only accept the short form.
   let success = U32.(res >^ 0ul) || (ilen = 0ul && is_short_form) in
 
-  // Short form is easy to parse.
+  // Short form is easy to parse and always succeeds.
   assert (U8.(b0 <^ 0x80uy) ==> res = (uint8_to_uint32 b0) /\ success);
   // TODO
-  //assert (U8.(b0 >^ 0x80uy /\ b0 <^ 0x85uy) /\
-          //(U32.v len > (U8.v b0) - 0x80) ==> U32.(res >=^ 0ul) /\ success);
+  assert ((U8.(b0 >^ 0x80uy /\ b0 <^ 0x85uy) /\ (U32.v len > ((U8.v b0) - 0x80))) ==> U32.(res >=^ 0ul)); //\ success);
 
   let h = ST.get() in
   // Fail when given a zero length in long form.
@@ -185,12 +202,28 @@ let parse_len buf len out_len =
   // The long form must have enough length bytes.
   assert (U8.(b0 >^ 0x80uy /\ b0 <^ 0x85uy) /\
           (U32.v len <= (U8.v b0) - 0x80) ==> res = 0ul /\ not success);
-  // The long form must not be all zero bytes. TODO
+
+  // TODO The long form must not be all zero bytes.
   //Seq.lemma_len_slice (as_seq h buf) 1 ((U8.v b0) - 0x80 + 1);
   //Seq.lemma_index_create ((U8.v b0) - 0x80) 0uy ((U8.v b0) - 0x80 - 1);
-  //assert (U8.(b0 >^ 0x80uy /\ b0 <^ 0x85uy) /\
-          //(U32.v len > (U8.v b0) - 0x80) /\
-          //(Seq.equal (Seq.slice (as_seq h buf) 1 ((U8.v b0) - 0x80 + 1)) (Seq.create ((U8.v b0) - 0x80) 0uy)) ==> res = 0ul /\ not success);
+  assert (U8.(b0 >^ 0x80uy /\ b0 <^ 0x85uy) ==> ((U8.v b0) - 0x80) == (U32.v ilen));
+  assert (U8.(b0 >^ 0x80uy /\ b0 <^ 0x85uy) ==> ((U8.v b0) - 0x80 + 1) == (U32.v ilen) + 1);
+  //assert ((U8.(b0 >^ 0x80uy /\ b0 <^ 0x85uy) /\ (U32.v len > ((U8.v b0) - 0x80)) /\ (Seq.equal (Seq.slice (as_seq h buf) 1 ((U8.v b0) - 0x80 + 1)) (Seq.create ((U8.v b0) - 0x80) 0uy))) ==> res = 0ul /\ not success);
+  assert (U8.(b0 >^ 0x80uy /\ b0 <^ 0x85uy) /\ (U32.v len > ((U8.v b0) - 0x80)) /\ res = 0ul ==> not success);
+  assert (U8.(b0 >^ 0x80uy /\ b0 <^ 0x85uy) /\ (U32.v len > ((U8.v b0) - 0x80)) /\ not success ==> Seq.length (Seq.slice (as_seq h buf) 1 ((U8.v b0) - 0x80 + 1)) == U32.v ilen);
+  assert (U8.(b0 >^ 0x80uy /\ b0 <^ 0x85uy) /\ (U32.v len > ((U8.v b0) - 0x80)) /\ not success ==> Seq.length (Seq.create ((U8.v b0) - 0x80) 0uy) == U32.v ilen);
+  //assert (U8.(b0 >^ 0x80uy /\ b0 <^ 0x85uy) /\ (U32.v len > ((U8.v b0) - 0x80)) /\ not success ==> (Seq.lemma_eq_intro (Seq.slice (as_seq h buf) 1 ((U8.v b0) - 0x80 + 1)) (Seq.create ((U8.v b0) - 0x80) 0uy)));
+  //assert (U8.(b0 >^ 0x80uy /\ b0 <^ 0x85uy) /\ (U32.v len > ((U8.v b0) - 0x80)) /\ not success ==> (Seq.equal (Seq.slice (as_seq h buf) 1 ((U8.v b0) - 0x80 + 1)) (Seq.create ((U8.v b0) - 0x80) 0uy)));
+  //assert (b0 = 0x81uy /\ (U32.v len > ((U8.v b0) - 0x80)) /\ not success ==> get h buf 1 == 0uy);
+  //assert (b0 = 0x82uy /\ (U32.v len > ((U8.v b0) - 0x80)) /\ not success ==> get h buf 1 == 0uy /\ get h buf 2 == 0uy);
+  //assert (b0 = 0x83uy /\ (U32.v len > ((U8.v b0) - 0x80)) /\ not success ==> get h buf 1 == 0uy /\ get h buf 2 == 0uy /\ get h buf 3 == 0uy);
+  //assert (b0 = 0x84uy /\ (U32.v len > ((U8.v b0) - 0x80)) /\ not success ==> get h buf 1 == 0uy /\ get h buf 2 == 0uy /\ get h buf 3 == 0uy /\ get h buf 4 == 0uy);
+  // TODO
+  //assert (b0 = 0x81uy /\ (U32.v len > ((U8.v b0) - 0x80)) /\ not success ==> Seq.equal (Seq.slice (as_seq h buf) 1 2) (Seq.create 1 0uy));
+  //assert (b0 = 0x81uy /\ (U32.v len > ((U8.v b0) - 0x80)) /\ not success ==> Seq.equal (Seq.slice (as_seq h buf) 1 2) (Seq.create ((U8.v b0) - 0x80) 0uy));
+  //assert (b0 = 0x81uy /\ (U32.v len > ((U8.v b0) - 0x80)) /\ not success ==> Seq.equal (Seq.slice (as_seq h buf) ((U8.v b0) - 0x80) 2) (Seq.create ((U8.v b0) - 0x80) 0uy));
+  //assert (b0 = 0x81uy /\ (U32.v len > ((U8.v b0) - 0x80)) /\ not success ==> Seq.equal (Seq.slice (as_seq h buf) ((U8.v b0) - 0x80) ((U8.v b0) - 0x80 + 1)) (Seq.create ((U8.v b0) - 0x80) 0uy));
+  //assert (U8.v b0 > 081 /\ (U32.v len > ((U8.v b0) - 0x80)) /\ not success ==> Seq.equal (Seq.slice (as_seq h buf) ((U8.v b0) - 0x80) ((U8.v b0) - 0x80 + 1)) (Seq.create ((U8.v b0) - 0x80) 0uy));
 
   // TODO check long form with starting zero bytes
 
